deps/poulet4/lib/Semantics.v
@@ -510,14 +510,16 @@ Inductive exec_expr (read_one_bit : option bool -> bool -> Prop)
                              (MkExpression tag (ExpTypeMember tname member) typ dir)
                              (ValBaseSenumField ename member sv)
   | exec_expr_error_member : forall err this st tag typ dir,
-                             exec_expr read_one_bit this st
-                             (MkExpression tag (ExpErrorMember err) typ dir)
-                             (ValBaseError err)
+      exec_expr
+        read_one_bit this st
+        (MkExpression tag (ExpErrorMember err) typ dir)
+        (ValBaseError err)
   | exec_expr_other_member : forall expr member sv sv' this st tag typ dir,
-                             exec_expr read_one_bit this st expr sv ->
-                             get_member sv member sv' ->
-                             exec_expr read_one_bit this st
-                             (MkExpression tag (ExpExpressionMember expr member) typ dir) sv'
+      exec_expr read_one_bit this st expr sv ->
+      get_member sv member sv' ->
+      exec_expr
+        read_one_bit this st
+        (MkExpression tag (ExpExpressionMember expr member) typ dir) sv'
   (* TODO:
      ValBaseHeader: setValid, setInvalid, isValid are supposed to be handled in exec_builtin
      ValBaseUnion: isValid is supposed to be handled in exec_builtin
@@ -533,14 +535,6 @@ Inductive exec_expr (read_one_bit : option bool -> bool -> Prop)
                           exec_expr read_one_bit this st
                           (MkExpression tag ExpDontCare typ dir)
                           ValBaseNull.
-(*with exec_exprs (read_one_bit : option bool -> bool -> Prop) : 
-                path -> state -> list (@Expression tags_t) -> list Sval -> Prop :=
-  | exec_exprs_nil : forall this st,
-                     exec_exprs read_one_bit this st nil nil
-  | exec_exprs_cons : forall this st expr es sv svs,
-                      exec_expr read_one_bit this st expr sv ->
-                      exec_exprs read_one_bit this st es svs ->
-                      exec_exprs read_one_bit this st (expr :: es) (sv :: svs).*)
 
 Inductive exec_expr_det (read_one_bit : option bool -> bool -> Prop) :
                         path -> (* temp_env -> *) state -> (@Expression tags_t) -> Val ->
@@ -845,7 +839,7 @@ Definition get_entries (s : state) (table : path) (const_entries : option (list 
 Inductive exec_match (read_one_bit : option bool -> bool -> Prop) : 
                      path -> state -> @Match tags_t -> ValSet -> Prop :=
   | exec_match_dont_care : forall this st tag typ,
-                           exec_match read_one_bit this st (MkMatch tag MatchDontCare typ) ValSetUniversal
+      exec_match read_one_bit this st (MkMatch tag MatchDontCare typ) ValSetUniversal
   | exec_match_mask : forall expr exprv mask maskv this st tag typ,
                       exec_expr_det read_one_bit this st expr exprv ->
                       exec_expr_det read_one_bit this st mask maskv ->
@@ -1391,12 +1385,12 @@ Inductive exec_builtin : path -> state -> Lval -> ident -> list Sval -> state ->
 Inductive exec_stmt (read_one_bit : option bool -> bool -> Prop) :
                     path -> state -> (@Statement tags_t) -> state -> signal -> Prop :=
   | exec_stmt_assign : forall lhs lv rhs v sv this_path st tags typ st' sig,
-                        exec_expr_det read_one_bit this_path st rhs v ->
-                        exec_lexpr read_one_bit this_path st lhs lv sig ->
-                        val_to_sval v sv -> 
-                        (if is_continue sig then exec_write this_path st lv sv st' else st' = st) ->
-                        exec_stmt read_one_bit this_path st
-                        (MkStatement tags (StatAssignment lhs rhs) typ) st' sig
+      exec_expr_det read_one_bit this_path st rhs v ->
+      exec_lexpr read_one_bit this_path st lhs lv sig ->
+      val_to_sval v sv -> 
+      (if is_continue sig then exec_write this_path st lv sv st' else st' = st) ->
+      exec_stmt read_one_bit this_path st
+                (MkStatement tags (StatAssignment lhs rhs) typ) st' sig
   | exec_stmt_assign_func_call : forall lhs lv rhs sv this_path st tags typ st' st'' sig sig' ret_sig,
                                  exec_call read_one_bit this_path st rhs st' sig' ->
                                  exec_lexpr read_one_bit this_path st lhs lv sig ->
